#+OPTIONS: toc:nil

\begin{flalign*}
& q_t + \sum_{i=1}^3 \frac{\partial F_i}{\partial x_i} = f \\
& q_t + \frac{\partial F_1}{\partial x} + \frac{\partial F_2}{\partial y} - f = 0 \\
& q_t + \frac{\partial F_1}{\partial x} + \frac{\partial F_2}{\partial y} + \sigma_1 q + \sigma_2 q + \sigma_3 q - f = 0 \\
& \int_{K_i}\left( q_t + \frac{\partial F_1}{\partial x} + \frac{\partial F_2}{\partial y} + \sigma_1 q + \sigma_2 q + \sigma_3 q - f \right) l \, dx = 0 \\
& \int_{K_i} \left( q_t - f \right) l \, dV - \int_{K_i} \left( \frac{\partial F_1}{\partial x} + \frac{\partial F_2}{\partial y} \right) l \, dV + \int_{K_i} \left( \sigma_1 q + \sigma_2 q + \sigma_3 q \right) l \, dV = 0 \\
& \int_{K_i} \left( q_t - f \right) l \, dV - \int_{K_i} \left( F_1 + F_2 \right) l \, dV + \int_{K_i} \left( \sigma_1 q + \sigma_2 q + \sigma_3 q \right) l \, dV = -\int_{\partial K_i} \left( n_1 F_1 + n_2 F_2 \right) l \, dS \\
& \end{flalign*}
